Fix completeness of the elimination restriction
This changes the handling of the elimination restriction in two ways:
1. The elimination restriction is now not checked if check_univs is false.
2. The elimination restriction was not complete when checking the Set
   restriction (only used for impredicative set in Coq). It is not
   enough to do a syntactic check on the universe since we could have
   constraints that force polymorphic universes to be Set. Instead, now
   the valuation is checked (in the specification) and the graph is
   consulted (in the checker). Coq has the same problem which I
   reported at https://github.com/coq/coq/issues/13465. This fixes that
   issue on the MetaCoq side.

template-coq/theories/EnvironmentTyping.v
@@ -635,7 +635,7 @@ Module DeclarationTyping (T : Term) (E : EnvironmentSig T)
         on_projs_noidx : #|ind_indices| = 0;
         (** The inductive cannot have indices *)
 
-        on_projs_elim : idecl.(ind_kelim) = InType;
+        on_projs_elim : idecl.(ind_kelim) = IntoAny;
         (** This ensures that all projections are definable *)
 
         on_projs_all : #|idecl.(ind_projs)| = context_assumptions (cshape_args cshape);
@@ -649,48 +649,43 @@ Module DeclarationTyping (T : Term) (E : EnvironmentSig T)
     (** This ensures that all sorts in kelim are lower
         or equal to the top elimination sort, if set.
         For inductives in Type we do not check [kelim] currently. *)
-
-    Fixpoint elim_sort_prop_ind ind_ctors_sort :=
+    
+    Definition elim_sort_prop_ind (ind_ctors_sort : list constructor_shape) :=
       match ind_ctors_sort with
-      | [] => (* Empty inductive proposition: *) InType
-      | [ s ] => match universe_family (cshape_sort s) with
-                | InProp => (* Not squashed: all arguments are in Prop  *)
-                  (* This is singleton elimination *) InType
-                | InSProp => (* Not squashed: all arguments are in SProp *)
-                  InType
-                | _ => (* Squashed: some arguments are higher than Prop,
-                        restrict to Prop *) InProp
-                end
-      | _ => (* Squashed: at least 2 constructors *) InProp
+      | [] => (* Empty inductive proposition: *) IntoAny
+      | [ s ] =>
+        if Universes.is_propositional (cshape_sort s) then
+          IntoAny (* Singleton elimination *)
+        else
+          IntoPropSProp (* Squashed: some arguments are higher than Prop, restrict to Prop *)
+      | _ => (* Squashed: at least 2 constructors *) IntoPropSProp
       end.
       
     Fixpoint elim_sort_sprop_ind (ind_ctors_sort : list constructor_shape) :=
       match ind_ctors_sort with
-      | [] => (* Empty inductive strict proposition: *) InType
-      | _ => (* All other inductives in SProp are squashed *) InSProp
+      | [] => (* Empty inductive strict proposition: *) IntoAny
+      | _ => (* All other inductives in SProp are squashed *) IntoSProp
       end.
 
     Definition check_ind_sorts (Σ : global_env_ext)
               params kelim ind_indices cshapes ind_sort : Type :=
-      match universe_family ind_sort with
-      | InProp =>
+      if Universe.is_prop ind_sort then
         (** The inductive is declared in the impredicative sort Prop *)
         (** No universe-checking to do: any size of constructor argument is allowed,
             however elimination restrictions apply. *)
-        leb_sort_family kelim (elim_sort_prop_ind cshapes)
-      | InSProp => 
+        allowed_eliminations_subset kelim (elim_sort_prop_ind cshapes)
+      else if Universe.is_sprop ind_sort then
         (** The inductive is declared in the impredicative sort SProp *)
         (** No universe-checking to do: any size of constructor argument is allowed,
             however elimination restrictions apply. *)
-        leb_sort_family kelim (elim_sort_sprop_ind cshapes)
-      | _ =>
+        allowed_eliminations_subset kelim (elim_sort_sprop_ind cshapes)
+      else
         (** The inductive is predicative: check that all constructors arguments are
             smaller than the declared universe. *)
         check_constructors_smaller Σ cshapes ind_sort
         × if indices_matter then
             type_local_ctx Σ params ind_indices ind_sort
-          else True
-      end.
+          else True.
 
     Record on_ind_body Σ mind mdecl i idecl :=
       { (** The type of the inductive must be an arity, sharing the same params
