pcuic/theories/PCUICInversion.v
@@ -178,7 +178,7 @@ Section Inversion.
         let params := firstn npar args in
         build_case_predicate_type ind mdecl idecl params u ps = Some pty ×
         Σ ;;; Γ |- p : pty ×
-        leb_sort_family (universe_family ps) (ind_kelim idecl) ×
+        is_allowed_elimination Σ ps (ind_kelim idecl) ×
         isCoFinite (ind_finite mdecl) = false ×
         Σ;;; Γ |- c : mkApps (tInd ind u) args ×
         map_option_out (build_branches_type ind mdecl idecl params u p)
